src/Axioms_Io.v
@@ -11,10 +11,10 @@ Import ListNotations.
 
 (** IO Axioms *)
 
-Definition doRemote_session (t:AnnoTerm) (pTo:Plc) (e:EvC) : EvC.
+Definition doRemote_session (t:Term) (pTo:Plc) (e:EvC) : EvC.
 Admitted.
 
-Definition parallel_vm_thread (l:Loc) (t:AnnoTerm) (p:Plc) (e:EvC) : EvC.
+Definition parallel_vm_thread (l:Loc) (t:Term) (p:Plc) (e:EvC) : EvC.
 Admitted.
 
 (*
@@ -25,10 +25,10 @@ Admitted.
 Definition shuffled_events (el1:list Ev) (el2:list Ev) : list Ev.
 Admitted.
 
-Definition cvm_events (t:AnnoTerm) (p:Plc) (e:Evidence) : list Ev.
+Definition cvm_events (t:Term) (p:Plc) (e:Evidence) : list Ev.
 Admitted.
 
-Definition cvm_evidence (t:AnnoTerm) (p:Plc) (e:EvC) : EvC.
+Definition cvm_evidence (t:Term) (p:Plc) (e:EvC) : EvC.
 Admitted.
 
 (*
@@ -36,12 +36,13 @@ Definition remote_trace (t:AnnoTerm) (p:Plc) : list Ev.
 Admitted.
 *)
 
+
 Axiom remote_LTS: forall t n et, 
-    lstar (conf t n et) (cvm_events t n et) (stop n (aeval t n et)).
+    lstar (conf t n et) (cvm_events (unanno t) n et) (stop n (aeval t n et)).
 
 
 Axiom remote_Evidence_Type_Axiom: forall t n bits et,
-    get_et (doRemote_session t n (evc bits et)) = aeval t n et.
+    get_et (doRemote_session t n (evc bits et)) = eval t n et.
 
 
 Axiom at_evidence : forall t (p:Plc) (e:EvC),
@@ -61,20 +62,25 @@ Axiom par_events : forall t p,
     parallel_vm_events t p = remote_trace t p.
 *)
 
+
+
 Axiom bpar_shuffle : forall x tr p t1 t2 et1 et2,
     lstar (conf t1 p et1) tr (stop p (aeval t1 p et1)) ->
     lstar (bp x (conf t1 p et1) (conf t2 p et2))
           (shuffled_events tr
-                           (cvm_events t2 p et2))
+                           (cvm_events (unanno t2) p et2))
           (bp x (stop p (aeval t1 p et1)) (stop p (aeval t2 p et2))).
 
-Axiom thread_bookend_peel: forall t p et etr l a tr,
-    lstar (conf t p et) tr (stop p (aeval t p et)) ->
+Axiom thread_bookend_peel: forall (t:AnnoTerm) p (*et*) etr l (a:Term) tr,
+    (*lstar (conf t p et) tr (stop p (aeval t p et)) -> *)
     ([cvm_thread_start l p a etr] ++ tr ++ [cvm_thread_end l] =
      (shuffled_events tr (cvm_events a p etr))
     ).
 
+
+(*
 Axiom wf_ec_preserved_remote: forall a n e,
     wf_ec e ->
-    well_formed_r_annt a ->
+    well_formed_r a ->
     wf_ec (doRemote_session a n e).
+*)
