src/Impl_vm.v
@@ -15,18 +15,18 @@ Require Import Maps.
 
 Fixpoint copland_compile (t:AnnoTermPar): CVM unit :=
   match t with
-  | aasp_par (n,_) a =>
-      e <- do_prim n a ;;
+  | aasp_par a =>
+      e <- do_prim a ;;
       put_ev e
-  | aatt_par (reqi,rpyi) q t' =>
+  | aatt_par q t' =>
     e <- get_ev ;;
-    e' <- doRemote t' q e reqi rpyi ;;
+    e' <- doRemote t' q e ;;
     put_ev e'
-  | alseq_par _ t1 t2 =>
+  | alseq_par t1 t2 =>
       copland_compile t1 ;;
       copland_compile t2
-  | abseq_par (x,y) sp t1 t2 =>
-    pr <- split_ev x sp ;;
+  | abseq_par sp t1 t2 =>
+    pr <- split_ev sp ;;
     let '(e1,e2) := pr in
     put_ev e1 ;;
     copland_compile t1 ;;
@@ -34,16 +34,16 @@ Fixpoint copland_compile (t:AnnoTermPar): CVM unit :=
     put_ev e2 ;;
     copland_compile t2 ;;
     e2r <- get_ev ;;
-    join_seq y e1r e2r
-  | abpar_par (x,y) loc sp t1 t2 =>
-    pr <- split_ev x sp ;;
+    join_seq e1r e2r
+  | abpar_par loc sp t1 t2 =>
+    pr <- split_ev sp ;;
     let '(e1,e2) := pr in
     start_par_thread loc t2 e2 ;;
     put_ev e1 ;;
     copland_compile t1 ;;
     e1r <- get_ev ;;
     e2r <- wait_par_thread loc t2 e2 ;;
-    join_par y e1r e2r
+    join_par e1r e2r
   end.
 
 Definition run_cvm (t:AnnoTermPar) st : cvm_st :=
