src/Helpers_VmSemantics.v
@@ -10,29 +10,31 @@ Require Import Coq.Program.Tactics Coq.Program.Equality.
 
 Set Nested Proofs Allowed.
 
-Lemma pl_immut : forall t e tr p,
-    well_formed_r t ->
+Lemma pl_immut : forall t e tr p i,
+    (*well_formed_r t -> *)
     st_pl
       (execSt
          (copland_compile t)
          {|
            st_ev := e;
            st_trace := tr;
-           st_pl := p |}) = p.
+           st_pl := p;
+           st_evid := i|}) = p.
 Proof.
   induction t; intros.
   -
-    destruct r.
     destruct a; (* asp *)
       try destruct a; (* asp params *)
       df;
       try reflexivity.
   -
-    do_wf_pieces.
+    (*
+    do_wf_pieces. *)
     repeat (df; try dohtac; df).   
     reflexivity.
   -
-    do_wf_pieces.
+    (*
+    do_wf_pieces. *)
     simpl in *.
     monad_unfold.
     repeat break_match;
@@ -43,18 +45,17 @@ Proof.
     assert (p = st_pl0).
     {
       edestruct IHt1.
-      eassumption.
       jkjk'.
     }
     assert (st_pl0 = st_pl).
     {
       edestruct IHt2.
-      eassumption.
       jkjk'.
     }
     congruence.
   -
-    do_wf_pieces.
+    (*
+    do_wf_pieces. *)
     annogo.
     df.
     
@@ -67,14 +68,13 @@ Proof.
     assert (p = st_pl0).
     {
       edestruct IHt1.
-      eassumption.
       jkjk'; eauto.     
     }
 
     assert (st_pl0 = st_pl).
     {     
       edestruct IHt2.
-      eassumption.
+
       jkjk'; eauto.
     }
 
@@ -83,14 +83,12 @@ Proof.
       assert (p = st_pl).
       {
         edestruct IHt1.
-        eassumption.
           jkjk'; eauto.
       }
 
       assert (st_pl = st_pl0).
       {
         edestruct IHt2.
-        eassumption.
           jkjk'; eauto.
       }
 
@@ -98,16 +96,13 @@ Proof.
     +
       symmetry.
       edestruct IHt1.
-      eassumption.
       jkjk'; eauto.
     +
       symmetry.
       edestruct IHt1.
-      eassumption.
       jkjk'; eauto.
 
   -
-    do_wf_pieces.
     annogo.
     df.
 
@@ -122,7 +117,6 @@ Proof.
     assert (p = st_pl).
     {
       edestruct IHt.
-      eassumption.
       jkjk'; eauto.     
     }
     congruence.   
@@ -131,38 +125,39 @@ Proof.
     assert (p = st_pl).
     {
       edestruct IHt.
-      eassumption.
       jkjk'; eauto.     
     }
     congruence. 
 Defined.
 
 Ltac do_pl_immut :=
-  let tac H H2 :=
+  let tac H :=
        erewrite <- pl_immut;
         [ unfold execSt;
           rewrite H;
-          reflexivity | 
-          apply H2] in
+          reflexivity (*| 
+          apply H2*)] in
       match goal with
       | [H: copland_compile ?t
                             {| st_ev := _;
                         st_trace := _;
-                        st_pl := ?p |} =
+                                    st_pl := ?p;
+                            st_evid := _|} =
             (_,
              {| st_ev := _;
                          st_trace := _;
-                         st_pl := ?p' |}),
-         H2: well_formed_r ?t |- _] =>
-        assert_new_proof_by (p' = p) ltac:(tac H H2)  
+                         st_pl := ?p'; st_evid := _ |})
+         (*H2: well_formed_r ?t*) |- _] =>
+        assert_new_proof_by (p' = p) ltac:(tac H)  
       end.
 
 Lemma st_congr :
-  forall st tr e p,
+  forall st tr e p i,
     st_ev st = e ->
     st_trace st = tr ->
     st_pl st = p ->
-    st =  {| st_ev := e; st_trace := tr; st_pl := p |}.
+    st_evid st = i ->
+    st =  {| st_ev := e; st_trace := tr; st_pl := p; st_evid := i |}.
 Proof.
   intros.
   subst; destruct st; auto.
@@ -171,23 +166,23 @@ Defined.
 Ltac anhl :=
   annogo;
   match goal with
-  | [H: well_formed_r ?a,
+  | [(*H: well_formed_r ?a, *)
      H2: copland_compile ?a _ = _,
      H3: copland_compile ?a _ = _,
-     IH: context[well_formed_r ?a -> _] |- _] =>
+     IH: context[(*well_formed_r ?a*) _ -> _] |- _] =>
     edestruct IH;
-    [apply H | 
+    [(*apply H | *)
      apply H2 | apply H3 | idtac]; clear H2; clear H3;
     destruct_conjs; subst
   end.
 
-Lemma hihi : forall t e e' e'' x x' y y' p p' p'',
-    well_formed_r t ->
-    copland_compile t {| st_ev := e; st_trace := x; st_pl := p |} =
-    (Some tt, {| st_ev := e'; st_trace := x'; st_pl := p' |}) ->
-    copland_compile t {| st_ev := e; st_trace := y; st_pl := p |} =
-    (Some tt, {| st_ev := e''; st_trace := y'; st_pl := p'' |}) ->
-    (e' = e'' /\ p' = p'').
+Lemma hihi : forall t e e' e'' x x' y y' p p' p'' i i' i'',
+    (*well_formed_r t -> *)
+    copland_compile t {| st_ev := e; st_trace := x; st_pl := p; st_evid := i |} =
+    (Some tt, {| st_ev := e'; st_trace := x'; st_pl := p'; st_evid := i' |}) ->
+    copland_compile t {| st_ev := e; st_trace := y; st_pl := p; st_evid := i |} =
+    (Some tt, {| st_ev := e''; st_trace := y'; st_pl := p''; st_evid := i'' |}) ->
+    (e' = e'' /\ p' = p'' /\ i' = i'').
 Proof.
   induction t; intros.
   - destruct a; (* asp *)
@@ -197,7 +192,7 @@ Proof.
     repeat (df; try dohtac; df).
     tauto.
   -
-    do_wf_pieces.
+    (*do_wf_pieces. *)
     df;
     repeat break_match;
     try (repeat find_inversion);
@@ -206,7 +201,8 @@ Proof.
     anhl.
     eauto. 
   -
-    do_wf_pieces.
+    (*
+    do_wf_pieces. *)
     df;
     repeat break_match;
     try (repeat find_inversion);
@@ -215,8 +211,9 @@ Proof.
     repeat anhl.
     repeat find_inversion.
     eauto.
-  - 
-    do_wf_pieces.
+  -
+    (*
+    do_wf_pieces. *)
     cbn in *.
     monad_unfold.
     repeat break_let.
@@ -245,14 +242,14 @@ Ltac clear_triv :=
 
 Ltac dohi'' :=
   annogo;
-  let tac Hwf H H' := eapply hihi; [apply Hwf | apply H | apply H'] in
+  let tac H H' := eapply hihi; [apply H | apply H'] in
   match goal with
-  | [H : copland_compile ?t1 {| st_ev := ?e; st_trace := _; st_pl := ?p |} =
-         (?opt, {| st_ev := ?e'; st_trace := _; st_pl := ?p' |}),
-         H' : copland_compile ?t1 {| st_ev := ?e; st_trace := _; st_pl := ?p |} =
-              (?opt, {| st_ev := ?e''; st_trace := _; st_pl := ?p'' |}),
-                Hwf : well_formed_r ?t1  |- _] =>
-    assert_new_proof_by (e' = e'' /\ p' = p'') ltac:(tac Hwf H H')
+  | [H : copland_compile ?t1 {| st_ev := ?e; st_trace := _; st_pl := ?p; st_evid := ?i |} =
+         (?opt, {| st_ev := ?e'; st_trace := _; st_pl := ?p'; st_evid := ?i' |}),
+         H' : copland_compile ?t1 {| st_ev := ?e; st_trace := _; st_pl := ?p; st_evid := ?i |} =
+              (?opt, {| st_ev := ?e''; st_trace := _; st_pl := ?p''; st_evid := ?i'' |})
+                (*Hwf : well_formed_r ?t1*)  |- _] =>
+    assert_new_proof_by (e' = e'' /\ p' = p'' /\ i' = i'') ltac:(tac H H')
   end.
 
 Ltac dohi :=
@@ -260,7 +257,7 @@ Ltac dohi :=
   repeat clear_triv.
 
 Lemma always_some : forall t vm_st vm_st' op,
-    well_formed_r t ->
+    (*well_formed_r t -> *)
     copland_compile 
       t
       vm_st =
@@ -276,26 +273,29 @@ Proof.
     repeat (df; try dohtac; df).
     tauto.
   -
-    df. 
-    do_wf_pieces.
+    df.
+    (*
+    do_wf_pieces. *)
     
     destruct o eqn:hhh;
       try (df; eauto).
   -
-    df.   
-    do_wf_pieces.
+    df.
+    (*
+    do_wf_pieces. *)
 
     repeat break_match;
       try (
           df; eauto).
   -
-    do_wf_pieces.
+    (*
+    do_wf_pieces. *)
     df.
     dohtac.
     df.
     simpl.
 
-    assert (o2 = Some tt) by eauto.
+    assert (o = Some tt) by eauto.
     subst.
     vmsts.
     df.
@@ -304,26 +304,26 @@ Defined.
 
 Ltac do_somett :=
   match goal with
-  | [H: copland_compile ?t _ = (?o, _),
-        H2: well_formed_r ?t |- _] =>
-    assert_new_proof_by (o = Some tt) ltac:(eapply always_some; [apply H2 | apply H])
+  | [H: copland_compile ?t _ = (?o, _)
+        (*H2: well_formed_r ?t*) |- _] =>
+    assert_new_proof_by (o = Some tt) ltac:(eapply always_some; [apply H])
   end.
 
 
 Ltac do_asome := repeat do_somett; repeat clear_triv.
 
-Lemma trace_irrel_pl : forall t tr1 tr1' tr2 e e' p1' p1,
-    well_formed_r t ->
+Lemma trace_irrel_pl : forall t tr1 tr1' tr2 e e' p1' p1 i i',
+    (*well_formed_r t -> *)
     copland_compile t
-           {| st_ev := e; st_trace := tr1; st_pl := p1 |} =
-    (Some tt, {| st_ev := e'; st_trace := tr1'; st_pl := p1' |}) ->
+           {| st_ev := e; st_trace := tr1; st_pl := p1; st_evid := i |} =
+    (Some tt, {| st_ev := e'; st_trace := tr1'; st_pl := p1'; st_evid := i' |}) ->
     
     st_pl
       (execSt (copland_compile t)
-           {| st_ev := e; st_trace := tr2; st_pl := p1 |}) = p1'.
+           {| st_ev := e; st_trace := tr2; st_pl := p1; st_evid := i |}) = p1'.
 Proof.
   intros.
-  destruct (copland_compile t {| st_ev := e; st_trace := tr2; st_pl := p1 |}) eqn:ff.
+  destruct (copland_compile t {| st_ev := e; st_trace := tr2; st_pl := p1; st_evid := i |}) eqn:ff.
   simpl.
   vmsts.
   simpl.
@@ -334,18 +334,40 @@ Proof.
   tauto.
 Defined.
 
-Lemma trace_irrel_ev : forall t tr1 tr1' tr2 e e' p1' p1,
-    well_formed_r t ->
+Lemma trace_irrel_ev : forall t tr1 tr1' tr2 e e' p1' p1 i i',
+    (*well_formed_r t -> *)
     copland_compile t
-           {| st_ev := e; st_trace := tr1; st_pl := p1 |} =
-    (Some tt, {| st_ev := e'; st_trace := tr1'; st_pl := p1' |}) ->
+           {| st_ev := e; st_trace := tr1; st_pl := p1; st_evid := i|} =
+    (Some tt, {| st_ev := e'; st_trace := tr1'; st_pl := p1'; st_evid := i' |}) ->
     
     st_ev
       (execSt (copland_compile t)
-           {| st_ev := e; st_trace := tr2; st_pl := p1 |}) = e'.
+           {| st_ev := e; st_trace := tr2; st_pl := p1; st_evid := i |}) = e'.
 Proof.
   intros.
-  destruct (copland_compile t {| st_ev := e; st_trace := tr2; st_pl := p1 |}) eqn:ff.
+  destruct (copland_compile t {| st_ev := e; st_trace := tr2; st_pl := p1; st_evid := i |}) eqn:ff.
+  simpl.
+  vmsts.
+  simpl.
+  do_asome.
+  subst.
+  dohi.
+  df.
+  tauto.
+Defined.
+
+Lemma trace_irrel_evid : forall t tr1 tr1' tr2 e e' p1' p1 i i',
+    (*well_formed_r t -> *)
+    copland_compile t
+           {| st_ev := e; st_trace := tr1; st_pl := p1; st_evid := i|} =
+    (Some tt, {| st_ev := e'; st_trace := tr1'; st_pl := p1'; st_evid := i' |}) ->
+    
+    st_evid
+      (execSt (copland_compile t)
+           {| st_ev := e; st_trace := tr2; st_pl := p1; st_evid := i |}) = i'.
+Proof.
+  intros.
+  destruct (copland_compile t {| st_ev := e; st_trace := tr2; st_pl := p1; st_evid := i |}) eqn:ff.
   simpl.
   vmsts.
   simpl.
