src/StVM.v
@@ -9,12 +9,16 @@ Require Import Maps.
 Require Import List.
 Import ListNotations.
 
+Definition Event_ID := nat.
+
 (* Specific VM monad state *)
 (*Definition ev_store := MapC nat EvidenceC. *)
 Record cvm_st : Type := mk_st
                           {st_ev:EvC ;
                            st_trace:list Ev ;
-                           st_pl:Plc (*;
+                           st_pl:Plc;
+                           st_evid:Event_ID
+                           (*;
                            st_store:ev_store*)}.
 
-Definition empty_vmst := mk_st (evc [] mt) [] 0 (* [] *) .
+Definition empty_vmst := mk_st (evc [] mt) [] 0 0 (* [] *) .
