src/VmSemantics.v
@@ -13,10 +13,10 @@ Import ListNotations.
 Require Import Coq.Program.Tactics Coq.Program.Equality.
 Require Import Coq.Arith.Peano_dec Lia.
 
-(*
-Set Nested Proofs Allowed.
- *)
 
+Set Nested Proofs Allowed.
+
+(*
 Lemma range_par: forall t,
     range_par t = range (unannoPar t).
 Proof.
@@ -36,6 +36,7 @@ Proof.
     repeat rewrite range_par in *;
     econstructor; eauto.
 Defined.
+*)
 
 Lemma anno_unanno_par: forall a l l' annt,
     anno_par a l = (l', annt) ->
@@ -64,6 +65,7 @@ Proof.
     congruence.
 Defined.
 
+(*
 Lemma fst_annopar: forall a a' l l',
     anno_par a l = (l', a') ->
     fst (range a) = fst (Term_Defs.range_par a').
@@ -417,24 +419,25 @@ Proof.
   }
   jkjke.
 Defined.
+*)
 
-Lemma st_trace_irrel : forall t tr1 tr1' tr2 tr2' e e' e'' p p' p'',
-    well_formed_r t ->
+Lemma st_trace_irrel : forall t tr1 tr1' tr2 tr2' e e' e'' p p' p'' i i' i'',
+    (*well_formed_r t -> *)
     copland_compile t
-           {| st_ev := e; st_trace := tr1; st_pl := p |} =
-    (Some tt, {| st_ev := e'; st_trace := tr1'; st_pl := p' |}) ->
+           {| st_ev := e; st_trace := tr1; st_pl := p; st_evid := i |} =
+    (Some tt, {| st_ev := e'; st_trace := tr1'; st_pl := p'; st_evid := i' |}) ->
 
     copland_compile t
-           {| st_ev := e; st_trace := tr2; st_pl := p |} =
-    (Some tt, {| st_ev := e''; st_trace := tr2'; st_pl := p'' |}) ->
+           {| st_ev := e; st_trace := tr2; st_pl := p; st_evid := i |} =
+    (Some tt, {| st_ev := e''; st_trace := tr2'; st_pl := p''; st_evid := i'' |}) ->
     
-    e' = e'' /\ p' = p''.
+    e' = e'' /\ p' = p'' /\ i' = i''.
 Proof.
   intros.
 
   assert (st_ev
       (execSt (copland_compile t)
-              {| st_ev := e; st_trace := tr2; st_pl := p |}) = e').
+              {| st_ev := e; st_trace := tr2; st_pl := p; st_evid := i |}) = e').
   eapply trace_irrel_ev; eauto.
   unfold execSt in *.
   subst''.
@@ -442,8 +445,16 @@ Proof.
 
   assert (st_pl
             (execSt (copland_compile t)
-                    {| st_ev := e; st_trace := tr2; st_pl := p |}) = p').
+                    {| st_ev := e; st_trace := tr2; st_pl := p; st_evid := i |}) = p').
   eapply trace_irrel_pl; eauto.
+  unfold execSt in *.
+  subst''.
+  simpl in *.
+
+  assert (st_evid
+            (execSt (copland_compile t)
+                    {| st_ev := e; st_trace := tr2; st_pl := p; st_evid := i |}) = i').
+  eapply trace_irrel_evid; eauto.
   unfold execSt in *.
   subst''.
   simpl in *.
@@ -453,23 +464,24 @@ Proof.
   repeat split; try congruence.
 Defined.
 
-Lemma alseq_decomp_gen : forall r t1' t2' e e'' p p'' init_tr tr,
-    well_formed_r (alseq_par r t1' t2') ->
-    copland_compile (alseq_par r t1' t2') {| st_ev := e; st_trace := init_tr; st_pl := p |} =
-    (Some tt, {| st_ev := e''; st_trace := tr; st_pl := p'' |}) ->
+Lemma alseq_decomp_gen : forall t1' t2' e e'' p p'' init_tr tr i i'',
+    (*well_formed_r (alseq_par r t1' t2') -> *)
+    copland_compile (alseq_par t1' t2') {| st_ev := e; st_trace := init_tr; st_pl := p; st_evid := i |} =
+    (Some tt, {| st_ev := e''; st_trace := tr; st_pl := p''; st_evid := i'' |}) ->
 
-    exists e' tr' p',
-      copland_compile t1' {| st_ev := e; st_trace := init_tr; st_pl := p |} =
-      (Some  tt, {| st_ev := e'; st_trace := tr'; st_pl := p' |}) /\
-        copland_compile t2' {| st_ev := e'; st_trace := tr'; st_pl := p' |} =
-        (Some tt, {| st_ev := e''; st_trace := tr; st_pl := p'' |}).     
+    exists e' tr' p' i',
+      copland_compile t1' {| st_ev := e; st_trace := init_tr; st_pl := p; st_evid := i |} =
+      (Some  tt, {| st_ev := e'; st_trace := tr'; st_pl := p'; st_evid := i' |}) /\
+        copland_compile t2' {| st_ev := e'; st_trace := tr'; st_pl := p'; st_evid := i' |} =
+        (Some tt, {| st_ev := e''; st_trace := tr; st_pl := p''; st_evid := i'' |}).     
 Proof.
-  intros.  
-  do_wf_pieces.
+  intros.
+  (*
+  do_wf_pieces. *)
   df.
   dosome.
   annogo.
-  exists st_ev. exists st_trace. exists st_pl.
+  exists st_ev. exists st_trace. exists st_pl. exists st_evid.
   split.
   reflexivity.
 
@@ -478,19 +490,19 @@ Defined.
 
 Ltac do_st_trace :=
   match goal with
-  | [H': context[{| st_ev := ?e; st_trace := ?tr; st_pl := ?p |}]
+  | [H': context[{| st_ev := ?e; st_trace := ?tr; st_pl := ?p; st_evid := ?i |}]
      |- context[?tr]] =>
     assert_new_proof_by
-      (tr = st_trace {| st_ev := e; st_trace := tr; st_pl := p |} )
+      (tr = st_trace {| st_ev := e; st_trace := tr; st_pl := p; st_evid := i |} )
       tauto
   end.
 
 Ltac do_st_trace_assumps :=
   match goal with
-  | [H': context[{| st_ev := ?e; st_trace := ?tr; st_pl := ?p |}]
+  | [H': context[{| st_ev := ?e; st_trace := ?tr; st_pl := ?p; st_evid := ?i |}]
      |- _] =>
     assert_new_proof_by
-      (tr = st_trace {| st_ev := e; st_trace := tr; st_pl := p |} )
+      (tr = st_trace {| st_ev := e; st_trace := tr; st_pl := p; st_evid := i |} )
       tauto
   end.
 
@@ -504,10 +516,10 @@ Ltac find_rw_in_goal :=
 Ltac cumul_ih :=
   match goal with
   | [H: context[(st_trace _ = _ ++ st_trace _)],
-        H': copland_compileP ?t1 {| st_ev := _; st_trace := ?m ++ ?k; st_pl := _ |}
+        H': copland_compileP ?t1 {| st_ev := _; st_trace := ?m ++ ?k; st_pl := _; st_evid := _ |}
                              (Some tt)
                              ?v_full,
-            H'': copland_compileP ?t1 {| st_ev := _; st_trace := ?k; st_pl := _ |}
+            H'': copland_compileP ?t1 {| st_ev := _; st_trace := ?k; st_pl := _; st_evid := _ |}
                                   (Some tt)
                                   ?v_suffix
      |- _] =>
@@ -515,28 +527,27 @@ Ltac cumul_ih :=
   end.
 
 Ltac wrap_ccp_dohi :=
-  do_wf_pieces;
+  (*do_wf_pieces; *)
   rewrite <- ccp_iff_cc in *;
   dd;
   dohi;
   rewrite ccp_iff_cc in *.
 
-Lemma st_trace_cumul' : forall t m k e p v_full v_suffix o_suffix,
-    well_formed_r t ->
+Lemma st_trace_cumul' : forall t m k e p v_full v_suffix o_suffix i,
+    (*well_formed_r t -> *)
 
     copland_compileP t
-               {| st_ev := e; st_trace := m ++ k; st_pl := p |}
+               {| st_ev := e; st_trace := m ++ k; st_pl := p; st_evid := i |}
                (Some tt) v_full ->
     
     copland_compileP t
-                     {| st_ev := e; st_trace := k; st_pl := p |}
+                     {| st_ev := e; st_trace := k; st_pl := p; st_evid := i |}
                      o_suffix v_suffix ->
 
     st_trace v_full = m ++ st_trace v_suffix.
 Proof.
   induction t; intros.
   -
-    destruct r.
     wrap_ccp.
     
     destruct a; (* asp *)
@@ -583,15 +594,15 @@ Proof.
 Defined.
 
 (* Instance of st_trace_cumul' where k=[] *)
-Lemma st_trace_cumul : forall t m e p v_full v_suffix o_suffix,
-    well_formed_r t ->
+Lemma st_trace_cumul : forall t m e p v_full v_suffix o_suffix i,
+    (*well_formed_r t -> *)
 
     copland_compileP t
-               {| st_ev := e; st_trace := m; st_pl := p |}
+               {| st_ev := e; st_trace := m; st_pl := p; st_evid := i |}
                (Some tt) v_full ->
     
     copland_compileP t
-                     {| st_ev := e; st_trace := []; st_pl := p |}
+                     {| st_ev := e; st_trace := []; st_pl := p; st_evid := i |}
                      o_suffix v_suffix ->
 
     st_trace v_full = m ++ st_trace v_suffix.
@@ -603,7 +614,7 @@ Proof.
 Defined.
 
 Lemma exists_some_cc: forall t st,
-    well_formed_r t ->
+    (*well_formed_r t -> *)
     exists st',
       copland_compile t st = (Some tt, st').
 Proof.
@@ -615,6 +626,13 @@ Proof.
 Defined.
 
 Ltac do_exists_some_cc t st :=
+    assert_new_proof_by
+      (exists st', copland_compile t st = (Some tt, st') )
+      ltac:(eapply exists_some_cc);
+    destruct_conjs.
+
+(*
+Ltac do_exists_some_cc t st :=
   match goal with
   | [H: well_formed_r t  |- _] =>
     assert_new_proof_by
@@ -622,23 +640,26 @@ Ltac do_exists_some_cc t st :=
       ltac:(eapply exists_some_cc; [apply H])
   end;
   destruct_conjs.
+*)
 
-Lemma suffix_prop : forall t e e' tr tr' p p',
-    well_formed_r t ->
+Lemma suffix_prop : forall t e e' tr tr' p p' i i',
+    (*well_formed_r t -> *)
     copland_compileP t
            {| st_ev := e;
               st_trace := tr;
-              st_pl := p |}
+              st_pl := p;
+              st_evid := i |}
            (Some tt)
            {|
              st_ev := e';
              st_trace := tr';
-             st_pl := p' |} ->
+             st_pl := p';
+             st_evid := i' |} ->
     exists l, tr' = tr ++ l.
 Proof.
   intros.
 
-  do_exists_some_cc t {| st_ev := e; st_trace := []; st_pl := p |}.
+  do_exists_some_cc t {| st_ev := e; st_trace := []; st_pl := p; st_evid := i |}.
 
   rewrite ccp_iff_cc in *.
 
@@ -647,11 +668,8 @@ Proof.
   eexists.
   unfold st_trace at 2.
   erewrite st_trace_cumul'.
-  2: {
-    eassumption.
-  }
   3: {
-    apply H2.
+    apply H1.
   }
   simpl.
   tauto.
@@ -662,33 +680,33 @@ Defined.
 Ltac do_suffix name :=
   match goal with
   | [H': copland_compileP ?t
-         {| st_ev := _; st_trace := ?tr; st_pl := _ |}
+         {| st_ev := _; st_trace := ?tr; st_pl := _; st_evid := _ |}
          (Some tt)
-         {| st_ev := _; st_trace := ?tr'; st_pl := _ |},
-         H2: well_formed_r ?t |- _] =>
+         {| st_ev := _; st_trace := ?tr'; st_pl := _; st_evid := _ |}
+         (*H2: well_formed_r ?t*) |- _] =>
     assert_new_proof_as_by
       (exists l, tr' = tr ++ l)
-      ltac:(eapply suffix_prop; [apply H2 | apply H'])
+      ltac:(eapply suffix_prop; [apply H'])
              name
   end.
 
-Lemma alseq_decomp : forall r t1' t2' e e'' p p'' tr,
-    well_formed_r (alseq_par r t1' t2') ->
-    copland_compileP (alseq_par r t1' t2')
-                     {| st_ev := e; st_trace := []; st_pl := p |}
+Lemma alseq_decomp : forall t1' t2' e e'' p p'' tr i i'',
+    (*well_formed_r (alseq_par r t1' t2') -> *)
+    copland_compileP (alseq_par t1' t2')
+                     {| st_ev := e; st_trace := []; st_pl := p; st_evid := i |}
                      (Some tt)
-                     {| st_ev := e''; st_trace := tr; st_pl := p'' |} ->
+                     {| st_ev := e''; st_trace := tr; st_pl := p''; st_evid := i'' |} ->
 
-    exists e' tr' p',
+    exists e' tr' p' i',
       copland_compileP t1'
-                       {| st_ev := e; st_trace := []; st_pl := p |}
+                       {| st_ev := e; st_trace := []; st_pl := p; st_evid := i |}
                        (Some  tt)
-                       {| st_ev := e'; st_trace := tr'; st_pl := p' |} /\
+                       {| st_ev := e'; st_trace := tr'; st_pl := p'; st_evid := i' |} /\
       exists tr'',
         copland_compileP t2'
-                         {| st_ev := e'; st_trace := []; st_pl := p' |}
+                         {| st_ev := e'; st_trace := []; st_pl := p'; st_evid := i' |}
                          (Some tt)
-                         {| st_ev := e''; st_trace := tr''; st_pl := p'' |} /\
+                         {| st_ev := e''; st_trace := tr''; st_pl := p''; st_evid := i'' |} /\
         tr = tr' ++ tr''.     
 Proof.
   intros.
@@ -697,12 +715,13 @@ Proof.
   eexists.
   eexists.
   eexists.
+  eexists.
 
   split.
   +
     eassumption.
   +
-    do_exists_some_cc t2' {| st_ev := st_ev0; st_trace := []; st_pl := st_pl0 |}.
+    do_exists_some_cc t2' {| st_ev := st_ev0; st_trace := []; st_pl := st_pl0; st_evid := st_evid0 |}.
     vmsts.
 
     eexists.
@@ -719,39 +738,39 @@ Proof.
         eassumption.
 Defined.
 
-Lemma restl : forall t e e' x tr p p',
-    well_formed_r t ->
+Lemma restl : forall t e e' x tr p p' i i',
+    (*well_formed_r t -> *)
     copland_compileP t
-                     {| st_ev := e; st_trace := x; st_pl := p |}
+                     {| st_ev := e; st_trace := x; st_pl := p; st_evid := i|}
                      (Some tt)
-                     {| st_ev := e'; st_trace := x ++ tr; st_pl := p' |} ->
+                     {| st_ev := e'; st_trace := x ++ tr; st_pl := p'; st_evid := i' |} ->
 
     copland_compileP t
-                     {| st_ev := e; st_trace := []; st_pl := p |}
+                     {| st_ev := e; st_trace := []; st_pl := p; st_evid := i |}
                      (Some tt)
-                     {| st_ev := e'; st_trace := tr; st_pl := p' |}.
+                     {| st_ev := e'; st_trace := tr; st_pl := p'; st_evid := i' |}.
 Proof.
   intros.
 
-  do_exists_some_cc t  {| st_ev := e; st_trace := []; st_pl := p |}.
+  do_exists_some_cc t  {| st_ev := e; st_trace := []; st_pl := p; st_evid := i |}.
   wrap_ccp_dohi.
 
   assert (st_trace = tr).
   {
     do_st_trace.
-    rewrite H1; clear H1.
+    rewrite H0; clear H0.
     assert (tr = st_trace).
     {
-      assert (StVM.st_trace {| st_ev := st_ev; st_trace := x ++ tr; st_pl := st_pl |} =
-              x ++ StVM.st_trace {| st_ev := st_ev; st_trace := st_trace; st_pl := st_pl |}).
+      assert (StVM.st_trace {| st_ev := st_ev; st_trace := x ++ tr; st_pl := st_pl; st_evid := st_evid|} =
+              x ++ StVM.st_trace {| st_ev := st_ev; st_trace := st_trace; st_pl := st_pl; st_evid := st_evid |}).
       {
-        eapply st_trace_cumul;
+        eapply st_trace_cumul; 
         eassumption.
       }
       simpl in *.
       eapply app_inv_head; eauto.
     }
-    rewrite H1; clear H1.
+    rewrite H0; clear H0.
     simpl.
     tauto.
   }
@@ -761,16 +780,16 @@ Defined.
 Ltac do_restl :=
   match goal with
   | [H: copland_compileP ?t
-        {| st_ev := ?e; st_trace := ?tr; st_pl := ?p |}
+        {| st_ev := ?e; st_trace := ?tr; st_pl := ?p; st_evid := ?i |}
         (Some tt)
-        {| st_ev := ?e'; st_trace := ?tr ++ ?x; st_pl := ?p' |},
-        H2: well_formed_r ?t |- _] =>
+        {| st_ev := ?e'; st_trace := ?tr ++ ?x; st_pl := ?p'; st_evid := ?i' |}
+        (*H2: well_formed_r ?t*) |- _] =>
     assert_new_proof_by
       (copland_compileP t
-                        {| st_ev := e; st_trace := []; st_pl := p |}
+                        {| st_ev := e; st_trace := []; st_pl := p; st_evid := i|}
                         (Some tt)
-                        {| st_ev := e'; st_trace := x; st_pl := p' |})
-      ltac:(eapply restl; [apply H2 | apply H])
+                        {| st_ev := e'; st_trace := x; st_pl := p'; st_evid := i' |})
+      ltac:(eapply restl; [apply H])
   end.
 
 Lemma splitEv_T_l_LEFT: forall e bits bits' es e0 sp,
@@ -853,19 +872,20 @@ Ltac do_t_at_zero t x :=
   destruct y;
   destruct y as [x].
 
-Ltac do_assert_remote t e p :=
+Ltac do_assert_remote t e p i :=
   assert (
       copland_compile t
-                      {| st_ev := e; st_trace := []; st_pl := p|} =
+                      {| st_ev := e; st_trace := []; st_pl := p; st_evid := i|} =
       (Some tt,
        {| st_ev := doRemote_session (unannoPar t) p e;
                    st_trace := cvm_events (unannoPar t) p (get_et e);
-                               st_pl := p
+                               st_pl := p;
+                                        st_evid := (i + event_id_span (unannoPar t))
        |})
     ) by
-    (eapply copland_compile_at;
-     eapply wfr_annt_implies_wfr_par;
-     [eassumption | econstructor; jkjke]).
+    (eapply copland_compile_at).
+     (*eapply wfr_annt_implies_wfr_par; 
+     [eassumption | econstructor; jkjke]). *)
 
 Ltac do_assert_unannoPar t x :=
   assert (t = unannoPar x) by
@@ -988,7 +1008,7 @@ Defined.
 
 Lemma par_evidence_r: forall a p s e et e2 e3 l,
     parallel_vm_thread l a p (splitEv_r s (evc e et)) = evc e2 e3 ->
-    e3 = (eval (unanno a) p (splitEv_T_r s et)).
+    e3 = (eval a p (splitEv_T_r s et)).
 Proof.
   intros.
 
@@ -996,9 +1016,10 @@ Proof.
   destruct s.
   destruct s; destruct s0;
     simpl in *;
-    
+
+    (*
     erewrite eval_aeval with (i:=0);
-    rewrite aeval_anno;
+    rewrite aeval_anno; *)
     try (unfold mt_evc in * );
     erewrite <- remote_Evidence_Type_Axiom;
     rewrite at_evidence;
@@ -1006,13 +1027,13 @@ Proof.
     jkjke.
 Defined.
 
-Lemma cvm_refines_lts_evidence : forall t tr tr' bits bits' et et' p p',
-    well_formed_r t ->
+Lemma cvm_refines_lts_evidence : forall t tr tr' bits bits' et et' p p' i i',
+    (*well_formed_r t -> *)
     copland_compileP t
-                     (mk_st (evc bits et) tr p)
+                     (mk_st (evc bits et) tr p i)
                      (Some tt)
-                     (mk_st (evc bits' et') tr' p') ->
-    et' = (Term_Defs.eval (unanno (unannoPar t)) p et).
+                     (mk_st (evc bits' et') tr' p' i') ->
+    et' = (Term_Defs.eval (unannoPar t) p et).
 Proof.
   intros.
   generalizeEverythingElse t.
@@ -1031,11 +1052,13 @@ Proof.
     (*
     destruct e. *)
     dd.
+
+    (*
     
     erewrite eval_aeval.
     
     
-    rewrite aeval_anno.
+    rewrite aeval_anno. *)
     erewrite <- remote_Evidence_Type_Axiom.
     jkjke.
 
@@ -1045,9 +1068,9 @@ Proof.
     subst.
 
     edestruct alseq_decomp.
-    eassumption.
+    (*
+    eassumption. *)
     eapply restl.
-    eassumption.
     eassumption.
     destruct_conjs.
 
@@ -1074,7 +1097,7 @@ Proof.
     destruct_conjs; subst.
     repeat do_restl.
 
-    assert (e = (eval (unanno (unannoPar t1)) p (splitEv_T_l s et))).
+    assert (e = (eval (unannoPar t1) p (splitEv_T_l s et))).
     {
       destruct s; destruct s.
       ++
@@ -1087,7 +1110,7 @@ Proof.
     }
     dd.
 
-    assert (e0 = (eval (unanno (unannoPar t2)) p (splitEv_T_r s et))).
+    assert (e0 = (eval (unannoPar t2)) p (splitEv_T_r s et)).
     {
       destruct s.
       destruct s0.
@@ -1110,7 +1133,7 @@ Proof.
     destruct_conjs; subst.
     repeat do_restl.
 
-    assert (e = (eval (unanno (unannoPar t)) p (splitEv_T_l s et))).
+    assert (e = (eval (unannoPar t)) p (splitEv_T_l s et)).
     {
       destruct s; destruct s.
       ++
@@ -1123,15 +1146,13 @@ Proof.
     }
     dd.
 
-    assert (e0 = (eval (unanno a) p (splitEv_T_r s et))).
+    assert (e0 = (eval t0 p (splitEv_T_r s et))).
     {
       eapply par_evidence_r; eauto.
     }
 
     find_rw_in_goal.
     tauto.
-    Unshelve.
-    eauto.
 Defined.
 
 (*
@@ -1307,40 +1328,97 @@ Proof.
     eauto. 
 Defined.
 
-Lemma cvm_refines_lts_event_ordering : forall t cvm_tr bits bits' et et' p p',
-    well_formed_r t ->
+Lemma cvm_spans: forall t e tr p i e' tr' p' i',
     copland_compileP t
-                     (mk_st (evc bits et) [] p)
+                     {| st_ev := e; st_trace := tr; st_pl := p; st_evid := i |}
                      (Some tt)
-                     (mk_st (evc bits' et') cvm_tr p') ->
-    lstar (conf (unannoPar t) p et) cvm_tr (stop p (aeval (unannoPar t) p et)).
+                     {|
+                       st_ev := e';
+                       st_trace := tr';
+                       st_pl := p';
+                       st_evid := i'
+                     |} ->
+    i' = i + event_id_span (unannoPar t).
 Proof.
-  intros t cvm_tr bits bits' et et' p p' H H'.
+Admitted.
+
+Lemma cvm_refines_lts_event_ordering : forall t atp annt cvm_tr bits bits' et et' p p' i i' loc,
+    anno_parP atp t loc ->
+    annoP annt t i ->
+    (*
+    well_formed_r_annt annt -> *)
+    copland_compileP atp
+                     (mk_st (evc bits et) [] p i)
+                     (Some tt)
+                     (mk_st (evc bits' et') cvm_tr p' i') ->
+    lstar (conf annt p et) cvm_tr (stop p (aeval annt p et)).
+Proof.
+  intros t atp annt cvm_tr bits bits' et et' p p' i i' loc annoParPH annPH H'.
   generalizeEverythingElse t.
   induction t; intros.
   
   - (* aasp case *)
-    rewrite <- ccp_iff_cc in *.
-    destruct a; (* asp *)
-      try destruct a; (* asp params *)
-      df;
-      econstructor; try (econstructor; reflexivity).
+    wrap_ccp.
+    invc annPH;
+      destruct a; df;   
+        repeat break_match; try solve_by_inversion;
+          try unfold tag_ASP in *;
+          df;
+          
+          econstructor; try (econstructor; reflexivity).
     
   - (* aatt case *)
+    wrap_ccp.
+
+    (*
     rewrite <- ccp_iff_cc in *.
-    destruct r.
-    repeat (df; try dohtac; df).
+    destruct r. 
+     *)
     
-    assert (lstar (conf a n et) (cvm_events a n et) (stop n (aeval a n et))).
+    repeat (df; try dohtac; df).
+
+    inv_annoparP.
+    invc annPH.
+    cbn in *.
+    repeat break_let.
+    assert (annoP a t (S i)).
     {
+      econstructor.
+      jkjke.
+    }
+    dd.
+
+    assert (t = unanno a) as H3.
+    {
+      invc H1.
+      rewrite anno_unanno.
+      tauto.
+    }
+    
+    assert (lstar (conf a n et) (cvm_events t n et) (stop n (aeval a n et))).
+    {
+      rewrite H3.
+
       apply remote_LTS.
     }
+
+    
+    assert (i = fst (i, S n0)) as H2 by tauto.
+    
+
+    rewrite H2 at 2.
+    rewrite H3.
+
+
+                                
     
     eapply lstar_tran.
     econstructor.
+    (*econstructor. *)
     simpl.
     eapply lstar_transitive.
     eapply lstar_strem.
+    rewrite <- H3.
     cbn.
     eassumption.
 
@@ -1349,22 +1427,64 @@ Proof.
     simpl.
     assert (et' = (aeval a n et)).
     {
+      rewrite <- eval_aeval.
       erewrite <- remote_Evidence_Type_Axiom.
-      jkjke.
+      rewrite <- H3.
+      rewrite H0.
+      tauto.
     }
-    subst.
+    rewrite <- H4.
+    rewrite <- H3.
+
+    assert ((S i) + event_id_span t = n0).
+    {
+      assert (event_id_span t = n0 - (S i)).
+      {
+        eapply span_range.
+        eassumption.
+      }
+      rewrite H5.
+      assert (n0 > (S i)).
+      {
+        eapply anno_mono.
+        eassumption.
+      }
+      lia.
+    }
+
+    assert ((i + 1 + event_id_span t) = (S i) + event_id_span t).
+    {
+      lia.
+    }
+    rewrite H6.
+    rewrite H5.
+    rewrite H0.
+    simpl.
+    
+    
+
     
     econstructor.
+
     apply stattstop.
     econstructor.
 
   -  (* alseq case *)
-    do_wf_pieces.
+    (*
+    do_wf_pieces. *)
+
+    invc annoParPH.
+    invc annPH.
+    dd.
+    do_annopar_redo.
+    do_annopar_redo.
+
+    
     edestruct alseq_decomp; eauto.
     destruct_conjs.
     destruct x.
 
-    wrap_ccp.
+    
  
     econstructor.
     econstructor.
@@ -1374,6 +1494,7 @@ Proof.
     
     eapply IHt1.
     eassumption.
+    econstructor; jkjke.
     eassumption.
 
     eapply lstar_silent_tran.
@@ -1381,11 +1502,107 @@ Proof.
 
     eapply IHt2. (*with (e:= x). *)
     eassumption.
-    assert (e = Term_Defs.eval (unanno (unannoPar t1)) p et).
+    econstructor; jkjke.
+    assert (e = Term_Defs.eval (unannoPar a) p et).
     eapply cvm_refines_lts_evidence; eauto.
+
 
     subst.
     rewrite <- eval_aeval.
+    assert (unannoPar a = unanno a1).
+    {
+      assert (unannoPar a = t1).
+      {
+        inversion Heqp0.
+        destruct (anno_par t1 loc) eqn: hi.
+        eapply anno_unanno_par.
+        rewrite H5.
+        simpl.
+        eassumption.
+      }
+      assert (unanno a1 = t1).
+      {
+        
+        erewrite <- anno_unanno.
+        rewrite Heqp2.
+        simpl.
+        tauto.
+      }
+      congruence.
+    }
+    rewrite <- H5.
+    assert (H0 = p).
+    { wrap_ccp.
+      tauto.
+    }
+    subst.
+    assert (H1 = i + event_id_span t1).
+    {
+
+      assert (t1 = unannoPar a).
+      {
+        destruct (anno_par t1 loc) eqn: hi.
+        erewrite anno_unanno_par.
+        reflexivity.
+        inversion Heqp0.
+        rewrite H0.
+        rewrite hi.
+        
+        simpl.
+        
+        tauto.
+      }
+     
+      rewrite H0.
+      eapply cvm_spans; eauto.
+
+    }
+    assert (n = i + event_id_span t1).
+    {
+      
+      Check span_range.
+      (*
+     : forall (t : Term) (i j : nat) (t' : AnnoTerm),
+       anno t i = (j, t') -> event_id_span t = j - i
+       *)
+      assert (event_id_span t1 = n - i).
+      {
+      
+        eapply span_range.
+        eassumption.
+      }
+      rewrite H6.
+      assert (n > i).
+      {
+        eapply anno_mono.
+        eassumption.
+      }
+      lia.
+
+    }
+    assert (n = H1) by congruence.
+    subst.
+    
+    eassumption.
+  -
+    
+    
+      
+        
+      
+        congruence.
+        apply hi.
+        rewrite H5.
+        
+        invc Heqp0.
+        jkjke.
+        eassumption.
+      Check anno_unanno_par.
+            
+      erewrite <- anno_unanno_par.
+      reflexivity.
+      Check anno_unanno. 
+      erewrite <- anno_unanno.
     
     eassumption.
 
